:PROPERTIES:
:ID:       e207e4c0-b3b4-4ee5-b891-bc3a56832fea
:NOTE_LEVEL: 1
:ROAM_ALIASES: "Boolesche Algebra"
:END:
#+title: Boolean Algebra
#+filetags: :@computerEngineering:@boat:

* Boolean Algebra
** Boolean Algebra Order of Operations
+ Parenthesis
+ Inverses
+ Product
+ Sums

 \( X = \overline{A} \cdot \overline{B} + B \cdot C\)
  
| A | B | C |   | \not A | \not C | \not(A)\cdot\not(C) | B \cdot C | \not(A)\cdot\not(C) + B \cdot C |
|---+---+---+---+-----+-----+-----------+-------+-------------------|
| 0 | 0 | 0 |   |   1 |   1 |         1 |     0 |                 1 |
| 0 | 0 | 1 |   |   1 |   0 |         0 |     0 |                 0 |
| 0 | 1 | 0 |   |   1 |   1 |         1 |     0 |                 1 |
| 0 | 1 | 1 |   |   1 |   0 |         0 |     1 |                 1 |
| 1 | 0 | 0 |   |   0 |   1 |         0 |     0 |                 0 |
| 1 | 0 | 1 |   |   0 |   0 |         0 |     0 |                 0 |
| 1 | 1 | 0 |   |   0 |   1 |         0 |     0 |                 0 |
| 1 | 1 | 1 |   |   0 |   0 |         0 |     1 |                 1 |

Circuit:
[[file:/home/steve/OrgVault/images/computerEnginnering/basic_circuit_example_with_and_and_or.png]]

** Optimization

Proof can be done Exhaustively through Truth Tables, showing by exhaustive proof that two circuits / expressions are identical.

Basic example:

[[file:/home/steve/OrgVault/images/computerEnginnering/simplification_of_circuits_basic_example.png]]

The same output
lower circuit:

+ Faster
+ Less Power
+ Less physical Space
+ Costs Less

** Identities of Boolean Algebra
+ [[id:51871534-24f3-4d0b-b6bb-ead8c18e4e2e][Mathematical Indentities]]

*** Proof by truthtable
|     | w/self             | w/inverse   | w/1         | w/0       |
|-----+--------------------+-------------+-------------+-----------|
| AND | A \cdot A = A          | A \cdot \not A = 0 | A \cdot 1 = A   | A \cdot 0 = 0 |
| OR  | A + A = A          | A + \not A = 1 | A + 1 = 1   | A + 0 = A |
| XOR | A \oplus A = 0          | A \oplus \not A = 1 | A \oplus 1 = \not A | A \oplus 0 = A |
|     |                    |             |             |           |
|     | (this is how you   |             |             |           |
|     | do it in assembly) |             |             |           |


| A | A \cdot A     | A \cdot \neg A   | A \cdot 1     | w/0       |
|---+-----------+-----------+-----------+-----------|
| 0 | 0 \cdot 0 = 0 | 1 \cdot 1 = 0 | 0 \cdot 1 = 0 | 0 \cdot 0 = 0 |
| 1 | 1 \cdot 1 = 1 | 1 \cdot 0 = 0 | 1 \cdot 1 = 1 | 1 \cdot 0 = 0 |
|   |           |           |           |           |

| A | A + A     | A + \neg A   | A + 1     | w/0       |
|---+-----------+-----------+-----------+-----------|
| 0 | 0 + 0 = 0 | 0 + 1 = 1 | 0 + 1 = 0 | 0 + 0 = 0 |
| 1 | 1 + 1 = 1 | 1 + 0 = 1 | 1 + 1 = 1 | 1 + 0 = 1 |
|   |           |           |           |           |


| A | B | XOR - Output |
|---+---+--------------|
| 0 | 0 |            0 |
| 0 | 1 |            1 |
| 1 | 0 |            1 |
| 1 | 1 |            0 |

*** Reasoning
These are our *"Red Flags"*. If we see any of them, that means we can move things around to simplify the expression and thus the given circuit.
Any time there is a constant, you know automatically that you can simplify and cancel something out.


** Properties of Boolean Algebra

*** Commutative Law:
A + B = B + A
A \cdot B = B \cdot A

*** Associative Law
A + (B + C) = (A + B) + C
A \cdot (B \cdot C) = (A \cdot B) \cdot C

*** Distributive Law
A \cdot (B + C) =  A \cdot B  +  C \cdot A
A +  B \cdot C  = (A + B) \cdot (A + C)

**** Proof by Truthtable
| A | B | C |   | (B + C) | A \cdot (B + C) | = | A \cdot B | A \cdot C | A \cdot B + A \cdot C |
|---+---+---+---+---------+-------------+---+-------+-------+---------------|
| 0 | 0 | 0 |   |       0 |           0 |   |     0 |     0 |             0 |
| 0 | 0 | 1 |   |       1 |           0 |   |     0 |     0 |             0 |
| 0 | 1 | 0 |   |       1 |           0 |   |     0 |     0 |             0 |
| 0 | 1 | 1 |   |       1 |           0 |   |     0 |     0 |             0 |
| 1 | 0 | 0 |   |       0 |           0 |   |     0 |     0 |             0 |
| 1 | 0 | 1 |   |       1 |           1 |   |     0 |     1 |             1 |
| 1 | 1 | 0 |   |       1 |           1 |   |     1 |     0 |             1 |
| 1 | 1 | 1 |   |       1 |           1 |   |     1 |     1 |             1 |

(the following only works in boolean algebra, but not regular algebra)

\begin{math}
 A + B \cdot C = (A + B) \cdot (A + C)

 = (A + B) \cdot A + (A + B) \cdot C 

 = A \cdot A + A \cdot B + A \cdot C + B \cdot C
 
 = A + A \cdot B + A \cdot C + B \cdot C \\

 add identity:

= A \cdot 1 + A \cdot C + B \cdot C \\

= A \cdot (1 + B + ) + B \cdot C

 \text{since there is a 1 in the parenthesis, the value inside will always be 1} \\
 
 = A \cdot 1 + B \cdot C \\

remove identity:

 = A + B \cdot C
\end{math}


*** DeMorgan's Law
\( \overline{A \cdot B} \ne \overline{A} \cdot \overline{B} \)

however:

\( \overline{A \cdot B} = \overline{A} + \overline{B} \)

as well as

\( \overline{A + B} = \overline{A} \cdot \overline{B} \)


| A | B | \( \overline{A \cdot B}\) |   | \not A | \not B | \( \overline{A} + \overline{B} \)     |
|---+---+-----------------------+---+-----+-----+-----------------------------------|
| 0 | 0 |                     1 |   |   1 |   1 |                                 1 |
| 0 | 1 |                     1 |   |   1 |   0 |                                 1 |
| 1 | 0 |                     1 |   |   0 |   1 |                                 1 |
| 1 | 1 |                     0 |   |   0 |   0 |                                 0 |



| A | B | \( \overline{A + B}\) |   | \not A | \not B | \( \overline{A} \cdot \overline{B} \) |
|---+---+-----------------------+---+-----+-----+-----------------------------------|
| 0 | 0 |                     1 |   |   1 |   1 |                                 1 |
| 0 | 1 |                     0 |   |   1 |   0 |                                 0 |
| 1 | 0 |                     0 |   |   0 |   1 |                                 0 |
| 1 | 1 |                     0 |   |   0 |   0 |                                 0 |


**** Visual Representation

[[file:/home/steve/OrgVault/images/computerEnginnering/de_morgans_theorem_example_circuit.png]]

*** Extra

+ \(A + \overline{A} \cdot B = A + B  \)
+ \(A + A \cdot B = A  \)
  + since
    + A \cdot 1 + A \cdot B
    + A \cdot (1 + B)
    + A \cdot 1
    + A
